\documentclass[a4paper,10pt]{article}

\usepackage{srcltx}%%->enable dvi fwd/rev-search
\usepackage[dvips]{graphicx}
\usepackage{amsmath}\usepackage{amsfonts}\usepackage{amssymb}
\usepackage{pstricks}\usepackage{pst-plot}
\usepackage{psfrag}%%->replace text in eps files with Latex text
\usepackage{float}%%->set figure placement
\usepackage{mathrsfs}%%->script font
\usepackage{natbib}

\include{preamble}
%


%opening
\title{Series convergence}
\author{Timothy D. Williams}

\begin{document}

\maketitle

\begin{abstract}
Reference: \cite{williams-porter2009}
\end{abstract}

\section{Series}
\begin{align}\label{Gmn-def}
G_{mn}^{(j)}
 &=\sum_{\a\in \mathscr{S}_j}B_j^{(2)}(\a)F_m^{(j)}(\a)F^{(j)}_n(\a).
\end{align}
In practice we truncate this series so there are only $N$ imaginary roots in $\mathscr{S}_{j}$,
\ie 
\begin{align}\label{Gmn-N}
G_{mn}^{(j)}(N)
 &=\sum_{\a\in \mathscr{S}^{(N)}_j}B_j^{(2)}(\a)F_m^{(j)}(\a)F^{(j)}_n(\a),
\end{align}
where $\mathscr{S}^{(N)}_j\subset \mathscr{S}_j$.

\begin{align}
 F_n^{(j)}(\a)&=\frac2{H_1}\int_{-H}^{-\sig_1}\varf^{(j)}(z,\a)
 \cC_{2n}\left(\frac{z+H}{H_1}\right)dz\notag\\
 &=2{\rm sech}(\g H_j)\int_0^1\cos(\K t)\cC_{2n}(t)dt\notag\\
 &=\frac{(-1)^n\Gamma(\b)}{\cosh(\g
H_j)}\left(\frac\K2\right)^{-\b}(2n+\b)J_{2n+\b}(\K),
\end{align}
where $\K=-\rmi\g H_2$.

Now let $\tilde \g_{j,r}=\rmi n\pi/H_{j}$, and
$\tilde\K_{j,r}=-\rmi\tilde\g_{j,r}H_{2}=r\pi H_{2}/H_{j}=r\pi /\hat H_{j}$ ($r=1,2,\ldots$). 
Then
\begin{subequations}
\begin{align}
B_j^{(2)}(\tilde\g_{j,r})&=\frac\rmi{r\pi},\\
J_{2n+\b}(\tilde\K_{j,r})
&=\sqrt{\frac2{\pi\tilde\K_{j,r} }}
\cos\left (\tilde\K_{j,r}-(2n+\b)\frac\pi2-\frac\pi4 \right)
\notag\\
&=(-1)^{n}r^{-1/2}\sqrt{\frac{2\hat H_{j}}{\pi^{2} }}
\cos\left(\tilde\K_{j,r}-\b'\right),\\
%\notag\\
%&=(-1)^{n}r^{-1/2}\sqrt{\frac1{2\pi^{2}\hat H_{j} }}
%\left(\rme^{\rmi(\tilde\K_{j,r}-\b')}+\rme^{-\rmi(\tilde\K_{j,r}-\b')}\right),\\
\b'&=\frac\pi2\left (\b+\frac12 \right).
\end{align}
\end{subequations}

Thus
\begin{subequations}
\begin{align}
F_n^{(j)}(\tilde \g_{j,r})&=
(-1)^{r}r^{-(2\b+1)/2}f_{j,n}(\b)\cos\left(\tilde\K_{j,r}-\b'\right),\\
f_{j,n}(\b)&=\Gamma(\b)(2n+\b)\left(\frac\pi{2\hat H_{j}}\right)^{-\b}
\sqrt{\frac{2\hat H_{j}}{\pi^{2} }},
\end{align}
\end{subequations}
and
\begin{align}\label{Gmn-app0}
\tilde G_{mn}^{(j)}(N)
 &=\sum_{r=1}^{N}B_j^{(2)}(\tilde\g_{j,r})F_m^{(j)}(\tilde\g_{j,r})F^{(j)}_n(\tilde\g_{j,r})
 \notag\\
 &=\frac\rmi\pi f_{j,n}(\b)f_{j,m}(\b)\sum_{r=1}^{N}r^{-s}
 \cos^{2}\left(\tilde\K_{j,r}-\b'\right).
 \end{align}
where $s=2(\b+1)$.
Therefore
\begin{align}\label{Gmn-app}
\tilde G_{mn}^{(j)}
&=\lim_{N\ar\infty}\tilde G_{mn}^{(j)}(N)
\notag\\
 &=\frac\rmi{2\pi} f_{j,n}(\b)f_{j,m}(\b)\sum_{r=1}^{\infty}r^{-s}
 \left (1+\re\left (\rme^{-2\rmi\b'} \rme^{2\rmi\pi r/\hat H_{j}}\right)\right)
\notag\\
 &=\frac\rmi{2\pi} f_{j,n}(\b)f_{j,m}(\b)
 \left ( \z(s)+\re\left (\rme^{-2\rmi\b'}{\rm Li}_{s} \left(\rme^{2\rmi\pi /\hat H_{j}}\right)\right)\right),
% \left (1+\re\left (\rme^{-2\rmi\b'} \rme^{2\rmi\pi r/\hat H_{j}}\right)\right)
 \end{align}
 where
\begin{align}
{\rm Li}_{s}(z)&=\sum_{r=1}^{\infty}\frac{z^{r}}{r^{s}}
\notag\\
&=\frac{z}{\G(s)}\int_{0}^{\infty}\frac{t^{s-1}\rme^{-t}}{1-z\rme^{-t}}\rmd t
\end{align}
is the polylogarithm function (??). This integral can be done very efficiently with Gauss-Laguerre quadrature. Also note that ${\rm Li}_{s}(1)=\z(s)$, which also implies that for $j=2$, when $\hat H_{2}=1$,
\begin{align}\label{Gmn-app}
\tilde G_{mn}^{(2)}
&=\frac\rmi{2\pi} f_{2,n}(\b)f_{2,m}(\b)\z(s)
 \left ( 1+\cos(2\b')\right),
 \notag\\
 &=\frac\rmi{\pi} f_{2,n}(\b)f_{2,m}(\b)\z(s)\cos^{2}(\b')
 \end{align}
 
 Finally we approximate
 \begin{align}
G_{mn}^{(j)}\approx G_{mn}^{(j)}(N)-\tilde G_{mn}^{(j)}(N)+ \tilde G_{mn}^{(j)},
\end{align}
which gives the summand in the series (\ref{Gmn-app0}) decays like $O(r^{-(s+1)})$.
This means it can be truncated at a much lower value of $N$.% For example

\bibliographystyle{jfm}
\bibliography{master}

\end{document}